Implementing some stack operations

ver2/stack_operation_instructions.v
@@ -68,17 +68,16 @@ Ltac ctx_independent_tac f :=
   unfold f;
   reflexivity.
 
+
 Definition evm_add (ctx : context) (args : list EVMWord) : EVMWord :=
   match args with
   | [a;b] => wplus a b
   | _ => WZero
   end.
-
 Lemma add_comm: commutative_op evm_add.
 Proof.
   comm_op_tac_trivial evm_add wplus_comm.
 Qed.
-
 Lemma add_ctx_ind: ctx_independent_op evm_add.
 Proof.
   ctx_independent_tac evm_add.
@@ -89,12 +88,10 @@ Definition evm_mul (ctx : context) (args : list EVMWord) : EVMWord :=
   | [a;b] => wmult a b
   | _ => WZero
   end.
-
 Lemma mul_comm: commutative_op evm_mul.
 Proof.
   comm_op_tac_trivial evm_mul wmult_comm.
 Qed.
-
 Lemma mul_ctx_ind: ctx_independent_op evm_mul.
 Proof.
   ctx_independent_tac evm_mul.
@@ -118,92 +115,192 @@ Definition evm_div (ctx : context) (args : list EVMWord) : EVMWord :=
   | [a;b] => wdiv a b
   | _ => WZero
   end.
-
 Lemma div_ctx_ind: ctx_independent_op evm_div.
 Proof.
   ctx_independent_tac evm_div.
 Qed.
 
 
-
 Definition evm_sdiv (ctx : context) (args : list EVMWord) : EVMWord :=
   WZero.
 
+
 Definition evm_mod (ctx : context) (args : list EVMWord) : EVMWord :=
-  WZero.
+  match args with
+  | [a;b] => wmod a b
+  | _ => WZero
+  end.
+  
+Lemma mod_ctx_ind: ctx_independent_op evm_mod.
+Proof.
+  ctx_independent_tac evm_mod.
+Qed.
+
 
 Definition evm_smod (ctx : context) (args : list EVMWord) : EVMWord :=
   WZero.
 
+
+
 Definition evm_addmod (ctx : context) (args : list EVMWord) : EVMWord :=
-  WZero.
+  match args with
+  | [a;b;c] => wmod (wplus a b) c
+  | _ => WZero
+  end.
+Lemma addmod_ctx_ind: ctx_independent_op evm_addmod.
+Proof.
+  ctx_independent_tac evm_addmod.
+Qed.
 
 Definition evm_mulmod (ctx : context) (args : list EVMWord) : EVMWord :=
-  WZero.
+  match args with
+  | [a;b;c] => wmod (wmult a b) c
+  | _ => WZero
+  end.
+Lemma mulmod_ctx_ind: ctx_independent_op evm_mulmod.
+Proof.
+  ctx_independent_tac evm_mulmod.
+Qed.
+
 
 Definition evm_exp (ctx : context) (args : list EVMWord) : EVMWord :=
   match args with
   | [a;b] => NToWord EVMWordSize (N.pow (wordToN a) (wordToN b))
   | _ => WZero
   end.
-  
+Lemma exp_ctx_ind: ctx_independent_op evm_exp.
+Proof.
+  ctx_independent_tac evm_exp.
+Qed.
+
 
 Definition evm_signextend (ctx : context) (args : list EVMWord) : EVMWord :=
   WZero.
+
 
 Definition evm_lt (ctx : context) (args : list EVMWord) : EVMWord :=
   match args with
   | [a;b] => if (N.ltb (wordToN a) (wordToN b)) then WOne else WZero
   | _ => WZero
   end.
+Lemma lt_ctx_ind: ctx_independent_op evm_lt.
+Proof.
+  ctx_independent_tac evm_lt.
+Qed.
+
 
 Definition evm_gt (ctx : context) (args : list EVMWord) : EVMWord :=
   match args with
   | [a;b] => evm_lt ctx [b; a]
   | _ => WZero
   end.
+Lemma gt_ctx_ind: ctx_independent_op evm_gt.
+Proof.
+  ctx_independent_tac evm_gt.
+Qed.
+
 
 Definition evm_slt (ctx : context) (args : list EVMWord) : EVMWord :=
   WZero.
 
+
 Definition evm_sgt (ctx : context) (args : list EVMWord) : EVMWord :=
   WZero.
+
 
 Definition evm_eq (ctx : context) (args : list EVMWord) : EVMWord :=
   match args with
   | [a;b] => if weqb a b then WOne else WZero
   | _ => WZero
   end.
+Lemma eq_comm: commutative_op evm_eq.
+Proof.
+unfold commutative_op. intros a b ctx.
+unfold evm_eq. 
+destruct (weqb a b) eqn: eq_weqb_a_b.
+- apply weqb_sound in eq_weqb_a_b.
+  symmetry in eq_weqb_a_b.
+  rewrite <- weqb_true_iff in eq_weqb_a_b.
+  rewrite -> eq_weqb_a_b.
+  reflexivity.
+- apply weqb_false in eq_weqb_a_b.
+  apply not_eq_sym in eq_weqb_a_b.
+  apply weqb_ne in eq_weqb_a_b.
+  rewrite -> eq_weqb_a_b.
+  reflexivity.
+Qed.
+Lemma eq_ctx_ind: ctx_independent_op evm_eq.
+Proof.
+  ctx_independent_tac evm_eq.
+Qed.
+
   
 Definition evm_iszero (ctx : context) (args : list EVMWord) : EVMWord :=
   match args with
   | [a] => evm_eq ctx [a; WZero]
   | _ => WZero
   end.
+Lemma iszero_ctx_ind: ctx_independent_op evm_iszero.
+Proof.
+  ctx_independent_tac evm_iszero.
+Qed.
+
 
 Definition evm_and (ctx : context) (args : list EVMWord) : EVMWord :=
   match args with
   | [a;b] => wand a b
   | _ => WZero
   end.
+Lemma and_comm: commutative_op evm_and.
+Proof.
+  comm_op_tac_trivial evm_and wand_comm.
+Qed.
+Lemma and_ctx_ind: ctx_independent_op evm_and.
+Proof.
+  ctx_independent_tac evm_and.
+Qed.
+
 
 Definition evm_or (ctx : context) (args : list EVMWord) : EVMWord :=
   match args with
   | [a;b] => wor a b
   | _ => WZero
   end.
+Lemma or_comm: commutative_op evm_or.
+Proof.
+  comm_op_tac_trivial evm_or wor_comm.
+Qed.
+Lemma or_ctx_ind: ctx_independent_op evm_or.
+Proof.
+  ctx_independent_tac evm_or.
+Qed.
+
 
 Definition evm_xor (ctx : context) (args : list EVMWord) : EVMWord :=
   match args with
   | [a;b] => wxor a b
   | _ => WZero
   end.
+Lemma xor_comm: commutative_op evm_xor.
+Proof.
+  comm_op_tac_trivial evm_xor wxor_comm.
+Qed.
+Lemma xor_ctx_ind: ctx_independent_op evm_xor.
+Proof.
+  ctx_independent_tac evm_xor.
+Qed.
+
 
 Definition evm_not (ctx : context) (args : list EVMWord) : EVMWord :=
   match args with
   | [a] => wnot a
   | _ => WZero
   end.
+Lemma not_ctx_ind: ctx_independent_op evm_not.
+Proof.
+  ctx_independent_tac evm_not.
+Qed.
+  
 
 Definition evm_byte (ctx : context) (args : list EVMWord) : EVMWord :=
   WZero.
@@ -291,23 +388,23 @@ Definition evm_stack_opm : stack_op_instr_map :=
   MUL |->i OpImp 2 evm_mul (Some mul_comm) (Some mul_ctx_ind);
   SUB |->i OpImp 2 evm_sub None (Some sub_ctx_ind);
   DIV |->i OpImp 2 evm_div None (Some div_ctx_ind);
-  SDIV |->i OpImp 2 evm_sdiv None None;
-  MOD |->i OpImp 2 evm_mod None None;
-  SMOD |->i OpImp 2 evm_smod None None;
-  ADDMOD |->i OpImp 3 evm_addmod None None;
-  MULMOD |->i  OpImp 3 evm_mulmod None None;
-  EXP |->i OpImp 2 evm_exp None None;
-  SIGNEXTEND  |->i OpImp 2 evm_signextend None None;
-  LT |->i OpImp 2 evm_lt None None;
-  GT  |->i OpImp 2 evm_gt None None;
-  SLT |->i OpImp 2 evm_slt None None;
-  SGT |->i  OpImp 2 evm_sgt None None;
-  EQ |->i OpImp 2 evm_eq None None;
-  ISZERO |->i OpImp  1 evm_iszero None None;
-  AND |->i OpImp 2 evm_and None None;
-  OR |->i OpImp 2  evm_or None None;
-  XOR |->i OpImp 2 evm_xor None None;
-  NOT |->i OpImp 1 evm_not  None None;
+  SDIV |->i OpImp 2 evm_sdiv None None; (*TODO*)
+  MOD |->i OpImp 2 evm_mod None (Some mod_ctx_ind);
+  SMOD |->i OpImp 2 evm_smod None None; (*TODO*)
+  ADDMOD |->i OpImp 3 evm_addmod None (Some addmod_ctx_ind);
+  MULMOD |->i  OpImp 3 evm_mulmod None (Some mulmod_ctx_ind);
+  EXP |->i OpImp 2 evm_exp None (Some exp_ctx_ind);
+  SIGNEXTEND  |->i OpImp 2 evm_signextend None None; (*TODO*)
+  LT |->i OpImp 2 evm_lt None (Some lt_ctx_ind);
+  GT  |->i OpImp 2 evm_gt None (Some gt_ctx_ind);
+  SLT |->i OpImp 2 evm_slt None None; (*TODO*)
+  SGT |->i  OpImp 2 evm_sgt None None; (*TODO*)
+  EQ |->i OpImp 2 evm_eq (Some eq_comm) (Some eq_ctx_ind);
+  ISZERO |->i OpImp  1 evm_iszero None (Some iszero_ctx_ind);
+  AND |->i OpImp 2 evm_and (Some and_comm) (Some and_ctx_ind);
+  OR |->i OpImp 2  evm_or (Some or_comm) (Some or_ctx_ind);
+  XOR |->i OpImp 2 evm_xor (Some xor_comm) (Some xor_ctx_ind);
+  NOT |->i OpImp 1 evm_not  None (Some not_ctx_ind);
   BYTE |->i OpImp 2 evm_byte None None;
   SHL |->i OpImp 2 evm_shl  None None;
   SHR |->i OpImp 2 evm_shr None None;
